AwsCryptographicMaterialProviders/dafny/AwsCryptographyKeyStore/Model/AwsCryptographyKeyStoreTypes.dfy
@@ -16,6 +16,10 @@ include "../../../../StandardLibrary/src/Index.dfy"
  
  // Begin Generated Types
  
+ datatype BranchKeyStatusResolutionInput = | BranchKeyStatusResolutionInput (
+ nameonly branchKeyIdentifier: string ,
+ nameonly grantTokens: Option<GrantTokenList>
+ )
  datatype CreateKeyInput = | CreateKeyInput (
  nameonly grantTokens: Option<GrantTokenList>
  )
@@ -62,6 +66,7 @@ include "../../../../StandardLibrary/src/Index.dfy"
  GetActiveBranchKey := [];
  GetBranchKeyVersion := [];
  GetBeaconKey := [];
+ BranchKeyStatusResolution := [];
 }
  ghost var CreateKeyStore: seq<DafnyCallEvent<CreateKeyStoreInput, Result<CreateKeyStoreOutput, Error>>>
  ghost var CreateKey: seq<DafnyCallEvent<CreateKeyInput, Result<CreateKeyOutput, Error>>>
@@ -69,6 +74,7 @@ include "../../../../StandardLibrary/src/Index.dfy"
  ghost var GetActiveBranchKey: seq<DafnyCallEvent<GetActiveBranchKeyInput, Result<GetActiveBranchKeyOutput, Error>>>
  ghost var GetBranchKeyVersion: seq<DafnyCallEvent<GetBranchKeyVersionInput, Result<GetBranchKeyVersionOutput, Error>>>
  ghost var GetBeaconKey: seq<DafnyCallEvent<GetBeaconKeyInput, Result<GetBeaconKeyOutput, Error>>>
+ ghost var BranchKeyStatusResolution: seq<DafnyCallEvent<BranchKeyStatusResolutionInput, Result<(), Error>>>
 }
  trait {:termination false} IKeyStoreClient
  {
@@ -186,6 +192,21 @@ include "../../../../StandardLibrary/src/Index.dfy"
  && ValidState()
  ensures GetBeaconKeyEnsuresPublicly(input, output)
  ensures History.GetBeaconKey == old(History.GetBeaconKey) + [DafnyCallEvent(input, output)]
+ 
+ predicate BranchKeyStatusResolutionEnsuresPublicly(input: BranchKeyStatusResolutionInput , output: Result<(), Error>)
+ // The public method to be called by library consumers
+ method BranchKeyStatusResolution ( input: BranchKeyStatusResolutionInput )
+ returns (output: Result<(), Error>)
+ requires
+ && ValidState()
+ modifies Modifies - {History} ,
+ History`BranchKeyStatusResolution
+ // Dafny will skip type parameters when generating a default decreases clause.
+ decreases Modifies - {History}
+ ensures
+ && ValidState()
+ ensures BranchKeyStatusResolutionEnsuresPublicly(input, output)
+ ensures History.BranchKeyStatusResolution == old(History.BranchKeyStatusResolution) + [DafnyCallEvent(input, output)]
  
 }
  datatype KeyStoreConfig = | KeyStoreConfig (
@@ -409,6 +430,26 @@ include "../../../../StandardLibrary/src/Index.dfy"
  History.GetBeaconKey := History.GetBeaconKey + [DafnyCallEvent(input, output)];
 }
  
+ predicate BranchKeyStatusResolutionEnsuresPublicly(input: BranchKeyStatusResolutionInput , output: Result<(), Error>)
+ {Operations.BranchKeyStatusResolutionEnsuresPublicly(input, output)}
+ // The public method to be called by library consumers
+ method BranchKeyStatusResolution ( input: BranchKeyStatusResolutionInput )
+ returns (output: Result<(), Error>)
+ requires
+ && ValidState()
+ modifies Modifies - {History} ,
+ History`BranchKeyStatusResolution
+ // Dafny will skip type parameters when generating a default decreases clause.
+ decreases Modifies - {History}
+ ensures
+ && ValidState()
+ ensures BranchKeyStatusResolutionEnsuresPublicly(input, output)
+ ensures History.BranchKeyStatusResolution == old(History.BranchKeyStatusResolution) + [DafnyCallEvent(input, output)]
+ {
+ output := Operations.BranchKeyStatusResolution(config, input);
+ History.BranchKeyStatusResolution := History.BranchKeyStatusResolution + [DafnyCallEvent(input, output)];
+}
+ 
 }
 }
  abstract module AbstractAwsCryptographyKeyStoreOperations {
@@ -513,4 +554,20 @@ include "../../../../StandardLibrary/src/Index.dfy"
  ensures
  && ValidInternalConfig?(config)
  ensures GetBeaconKeyEnsuresPublicly(input, output)
+
+
+ predicate BranchKeyStatusResolutionEnsuresPublicly(input: BranchKeyStatusResolutionInput , output: Result<(), Error>)
+ // The private method to be refined by the library developer
+
+
+ method BranchKeyStatusResolution ( config: InternalConfig , input: BranchKeyStatusResolutionInput )
+ returns (output: Result<(), Error>)
+ requires
+ && ValidInternalConfig?(config)
+ modifies ModifiesInternalConfig(config)
+ // Dafny will skip type parameters when generating a default decreases clause.
+ decreases ModifiesInternalConfig(config)
+ ensures
+ && ValidInternalConfig?(config)
+ ensures BranchKeyStatusResolutionEnsuresPublicly(input, output)
 }
