AwsCryptographicMaterialProviders/dafny/AwsCryptographyKeyStore/test/TestKeyResolution.dfy
@@ -1,0 +1,108 @@
+// Copyright Amazon.com Inc. or its affiliates. All Rights Reserved.
+// SPDX-License-Identifier: Apache-2.0
+
+include "../src/Index.dfy"
+include "../src/CreateKeys.dfy"
+include "../src/KeyResolution.dfy"
+
+module TestKeyResolution {
+  import Types = AwsCryptographyKeyStoreTypes
+  import ComAmazonawsKmsTypes
+  import KMS = Com.Amazonaws.Kms
+  import DDB = Com.Amazonaws.Dynamodb
+  import DDBTypes = ComAmazonawsDynamodbTypes
+  import KMSTypes = ComAmazonawsKmsTypes
+  import KeyStore
+  import UUID
+  import Time
+  import opened StandardLibrary
+  import opened Wrappers
+  import opened AwsKmsUtils
+  import opened CreateKeys
+  import opened KeyResolution
+  
+  const branchKeyStoreName := "KeyStoreTestTable";
+  // THESE ARE TESTING RESOURCES DO NOT USE IN A PRODUCTION ENVIRONMENT
+  const keyArn := "arn:aws:kms:us-west-2:370957321024:key/9d989aa2-2f9c-438c-a745-cc57d3ad0126";
+
+  method {:test} TestActiveBranchKeyResolution() {
+    var kmsClient :- expect KMS.KMSClient();
+    var ddbClient :- expect DDB.DynamoDBClient();
+    var keyStoreConfig := Types.KeyStoreConfig(
+      id := None,
+      kmsKeyArn := keyArn,
+      ddbTableName := branchKeyStoreName,
+      ddbClient := Some(ddbClient),
+      kmsClient := Some(kmsClient)
+    );
+
+    var keyStore :- expect KeyStore.KeyStore(keyStoreConfig);
+
+    // Create a new key
+    // We will create a use this new key per run to avoid tripping up
+    // when running in different runtimes across different hosts
+    var branchKeyIdentifier :- expect keyStore.CreateKey(Types.CreateKeyInput(
+      grantTokens := None
+    ));
+    
+    WriteActiveActiveBranchKey(branchKeyIdentifier.branchKeyIdentifier, kmsClient, ddbClient);
+
+    // Resolve active key to latest key based on lexicographically timestamp value
+    var resolveActiveKeyResult := keyStore.BranchKeyStatusResolution(Types.BranchKeyStatusResolutionInput(
+      branchKeyIdentifier := branchKeyIdentifier.branchKeyIdentifier,
+      grantTokens := None
+    ));
+
+    expect resolveActiveKeyResult.Success?;
+  }
+
+  method WriteActiveActiveBranchKey(branchKeyIdentifer: string, kmsClient: KMSTypes.IKMSClient, ddbClient: DDBTypes.IDynamoDBClient) 
+    requires kmsClient.ValidState() && ddbClient.ValidState()
+    modifies ddbClient.Modifies, kmsClient.Modifies
+    ensures ddbClient.ValidState() && kmsClient.ValidState()
+  {
+
+    // DO NOT use the KeyStore methods this way
+    // We are doing this in order to continuously test that the APIs work
+    // as spec'd out.
+    
+    // In order to be able to test this again in ci we will deliberately
+    // add another active key under this branch key id
+    var timestamp := Time.GetCurrentTimeStamp();
+    var version := UUID.GenerateUUID();
+    expect timestamp.Success? && version.Success?;
+
+    var activeActiveBranchKeyEncryptionContext := activeBranchKeyEncryptionContext(
+      branchKeyIdentifer,
+      version.value,
+      timestamp.value,
+      branchKeyStoreName,
+      keyArn
+    );
+
+    var grantTokens := GetValidGrantTokens(None);
+    var maybeActiveActiveBranchKeyWithoutPlaintext := GenerateKey(
+      activeActiveBranchKeyEncryptionContext,
+      keyArn,
+      grantTokens.value,
+      kmsClient
+    );
+
+    expect maybeActiveActiveBranchKeyWithoutPlaintext.Success?;
+    var activeActiveBranchKeyWithoutPlaintext := maybeActiveActiveBranchKeyWithoutPlaintext.value;
+
+    expect activeActiveBranchKeyWithoutPlaintext.CiphertextBlob.Some?;
+    var activeActiveBranchKeyDDBMap := ToBranchKeyItemAttributeMap(
+      activeActiveBranchKeyEncryptionContext,
+      activeActiveBranchKeyWithoutPlaintext.CiphertextBlob.value
+    );
+
+    var writeActiveActiveBranchKey := WriteDecryptOnlyBranchKeys(
+      [activeActiveBranchKeyDDBMap],
+      branchKeyStoreName,
+      ddbClient
+    );
+
+    expect writeActiveActiveBranchKey.Success?;
+  }
+}
